<?xml version="1.0"?>


<!DOCTYPE rdf:RDF [
    <!ENTITY owl "http://www.w3.org/2002/07/owl#" >
    <!ENTITY obo "http://purl.obolibrary.org/obo/" >
    <!ENTITY xsd "http://www.w3.org/2001/XMLSchema#" >
    <!ENTITY xml "http://www.w3.org/XML/1998/namespace" >
    <!ENTITY rdfs "http://www.w3.org/2000/01/rdf-schema#" >
    <!ENTITY rdf "http://www.w3.org/1999/02/22-rdf-syntax-ns#" >
]>


<rdf:RDF xmlns="&obo;GENEPIO/imports/pto_import.owl#"
     xml:base="&obo;GENEPIO/imports/pto_import.owl"
     xmlns:rdf="http://www.w3.org/1999/02/22-rdf-syntax-ns#"
     xmlns:owl="http://www.w3.org/2002/07/owl#"
     xmlns:xml="http://www.w3.org/XML/1998/namespace"
     xmlns:xsd="http://www.w3.org/2001/XMLSchema#"
     xmlns:rdfs="http://www.w3.org/2000/01/rdf-schema#"
     xmlns:obo="http://purl.obolibrary.org/obo/">
    <owl:Ontology rdf:about="&obo;GENEPIO/imports/pto_import.owl"/>
    


    <!-- 
    ///////////////////////////////////////////////////////////////////////////////////////
    //
    // Annotation properties
    //
    ///////////////////////////////////////////////////////////////////////////////////////
     -->

    


    <!-- http://purl.obolibrary.org/obo/IAO_0000115 -->

    <!-- <owl:AnnotationProperty rdf:about="&obo;IAO_0000115">
        <obo:IAO_0000115 xml:lang="en">The official definition, explaining the meaning of a class or property. Shall be Aristotelian, formalized and normalized. Can be augmented with colloquial definitions.</obo:IAO_0000115>
        <rdfs:label xml:lang="en">definition</rdfs:label>
        <rdfs:label rdf:datatype="&xsd;string">definition</rdfs:label>
    </owl:AnnotationProperty> -->
    


    <!-- http://purl.obolibrary.org/obo/IAO_0000412 -->

    <!-- <owl:AnnotationProperty rdf:about="&obo;IAO_0000412">
        <rdfs:label xml:lang="en">imported from</rdfs:label>
    </owl:AnnotationProperty> -->
    


    <!-- http://www.w3.org/2000/01/rdf-schema#label -->

    <!-- <owl:AnnotationProperty rdf:about="&rdfs;label"/> -->
    


    <!-- 
    ///////////////////////////////////////////////////////////////////////////////////////
    //
    // Classes
    //
    ///////////////////////////////////////////////////////////////////////////////////////
     -->

    


    <!-- http://purl.obolibrary.org/obo/PCO_0000033 -->

    <owl:Class rdf:about="&obo;PCO_0000033">
        <obo:IAO_0000115 xml:lang="en">A type of social behavior in which a collection of humans intentionally gathers together on a temporary basis to engage socially.</obo:IAO_0000115>
        <obo:IAO_0000412 rdf:resource="&obo;pco.owl"/>
        <rdfs:label xml:lang="en">human social gathering activity</rdfs:label>
    </owl:Class>
    


    <!-- http://purl.obolibrary.org/obo/PCO_0000034 -->

    <owl:Class rdf:about="&obo;PCO_0000034">
        <rdfs:subClassOf rdf:resource="&obo;PCO_0000033"/>
        <obo:IAO_0000115 xml:lang="en">A human social event in which humans living in the same area or neighborhood gather to carry out activiites relevent to the people living in the area.</obo:IAO_0000115>
        <obo:IAO_0000412 rdf:resource="&obo;pco.owl"/>
        <rdfs:label xml:lang="en">human community event</rdfs:label>
    </owl:Class>
    


    <!-- http://purl.obolibrary.org/obo/PCO_0000035 -->

    <owl:Class rdf:about="&obo;PCO_0000035">
        <rdfs:subClassOf rdf:resource="&obo;PCO_0000033"/>
        <obo:IAO_0000115 xml:lang="en">A human social gathering in which the intention is to have a good time. Often the intention is to celebrate something like a birthday, anniversary, or holiday, but there is not always a purpose.</obo:IAO_0000115>
        <obo:IAO_0000412 rdf:resource="&obo;pco.owl"/>
        <rdfs:label xml:lang="en">party</rdfs:label>
    </owl:Class>
    


    <!-- http://purl.obolibrary.org/obo/PCO_0000037 -->

    <owl:Class rdf:about="&obo;PCO_0000037">
        <rdfs:subClassOf rdf:resource="&obo;PCO_0000033"/>
        <obo:IAO_0000412 rdf:resource="&obo;pco.owl"/>
        <rdfs:label xml:lang="en">potluck</rdfs:label>
    </owl:Class>
    


    <!-- http://purl.obolibrary.org/obo/PCO_0000038 -->

    <owl:Class rdf:about="&obo;PCO_0000038">
        <rdfs:subClassOf rdf:resource="&obo;PCO_0000033"/>
        <obo:IAO_0000115 xml:lang="en">A human social gathering at which two people are married. May include a legal or social ceremony.</obo:IAO_0000115>
        <obo:IAO_0000412 rdf:resource="&obo;pco.owl"/>
        <rdfs:label xml:lang="en">wedding</rdfs:label>
    </owl:Class>
    


    <!-- http://purl.obolibrary.org/obo/PCO_0000039 -->

    <owl:Class rdf:about="&obo;PCO_0000039">
        <rdfs:subClassOf rdf:resource="&obo;PCO_0000033"/>
        <obo:IAO_0000115 xml:lang="en">A human social gathering at which the key participant is an expectant parent and other guests bring presents for the soon to be born baby.</obo:IAO_0000115>
        <obo:IAO_0000412 rdf:resource="&obo;pco.owl"/>
        <rdfs:label xml:lang="en">baby shower</rdfs:label>
    </owl:Class>
</rdf:RDF>



<!-- Generated by the OWL API (version 4.2.6) https://github.com/owlcs/owlapi -->

